RocqOfRust/revm/revm_interpreter/instructions/tests/tx_info.v
@@ -1,0 +1,33 @@
+Require Import simulate.RocqOfRust.
+Require Import revm.revm_interpreter.instructions.simulate.tx_info.gasprice.
+Require Import revm.revm_interpreter.links.interpreter.
+Require Import revm.revm_interpreter.tests.host.
+Require Import revm.revm_interpreter.tests.interpreter.
+Require Import revm.revm_interpreter.tests.interpreter_types.
+Require Import ruint.links.lib.
+
+(** ** GASPRICE tests *)
+
+(** Test that GASPRICE pushes the effective gas price (= 42) onto the stack *)
+Goal
+  let stack := {| Stack.value := [] |} in
+  let interpreter := make_interpreter stack in
+  let host : TestHost.t := TestHost.Make in
+  let '(result_interpreter, _) := gasprice interpreter host in
+  result_interpreter.(Interpreter.stack).(Stack.value) = [{| Uint.value := 42 |}].
+Proof.
+  timeout 1 vm_compute.
+  reflexivity.
+Qed.
+
+(** Test that GASPRICE does not set an error *)
+Goal
+  let stack := {| Stack.value := [] |} in
+  let interpreter := make_interpreter stack in
+  let host : TestHost.t := TestHost.Make in
+  let '(result_interpreter, _) := gasprice interpreter host in
+  result_interpreter.(Interpreter.control).(Control.instruction_result) = None.
+Proof.
+  timeout 1 vm_compute.
+  reflexivity.
+Qed.
